Added termination proof for widening

src/HOL/IMP/Abs_Int2.thy
@@ -4,7 +4,6 @@ theory Abs_Int2
 imports Abs_Int1_ivl
 begin
 
-
 subsection "Widening and Narrowing"
 
 class WN = SL_top +
@@ -15,6 +14,8 @@ fixes narrow :: "'a \<Rightarrow> 'a \<Rightarrow> 'a" (infix "\<triangle>" 65)
 assumes narrow1: "y \<sqsubseteq> x \<Longrightarrow> y \<sqsubseteq> x \<triangle> y"
 assumes narrow2: "y \<sqsubseteq> x \<Longrightarrow> x \<triangle> y \<sqsubseteq> x"
 
+
+subsubsection "Intervals"
 
 instantiation ivl :: WN
 begin
@@ -37,6 +38,9 @@ proof qed
   (auto simp add: widen_ivl_def narrow_ivl_def le_option_def le_ivl_def empty_def split: ivl.split option.split if_splits)
 
 end
+
+
+subsubsection "Abstract State"
 
 instantiation st :: (WN)WN
 begin
@@ -63,6 +67,9 @@ next
 qed
 
 end
+
+
+subsubsection "Option"
 
 instantiation option :: (WN)WN
 begin
@@ -94,6 +101,9 @@ qed
 
 end
 
+
+subsubsection "Annotated commands"
+
 fun map2_acom :: "('a \<Rightarrow> 'a \<Rightarrow> 'a) \<Rightarrow> 'a acom \<Rightarrow> 'a acom \<Rightarrow> 'a acom" where
 "map2_acom f (SKIP {a1}) (SKIP {a2}) = (SKIP {f a1 a2})" |
 "map2_acom f (x ::= e {a1}) (x' ::= e' {a2}) = (x ::= e {f a1 a2})" |
@@ -121,25 +131,52 @@ by(induct y x rule: le_acom.induct) (simp_all add: narrow1)
 lemma narrow2_acom: "y \<sqsubseteq> x \<Longrightarrow> x \<triangle>\<^sub>c y \<sqsubseteq> x"
 by(induct y x rule: le_acom.induct) (simp_all add: narrow2)
 
+(*
+lemma strip_widen_acom:
+  "strip c' = strip (c::'a::WN acom) \<Longrightarrow>  strip (c \<nabla>\<^sub>c c') = strip c"
+by(induction "widen::'a\<Rightarrow>'a\<Rightarrow>'a" c c' rule: map2_acom.induct) simp_all
+
+lemma annos_widen_acom[simp]: "strip c1 = strip (c2::'a::WN acom) \<Longrightarrow>
+  annos(c1 \<nabla>\<^sub>c c2) = map (%(x,y).x\<nabla>y) (zip (annos c1) (annos(c2::'a::WN acom)))"
+by(induction "widen::'a\<Rightarrow>'a\<Rightarrow>'a" c1 c2 rule: map2_acom.induct)
+  (simp_all add: size_annos_same2)
+*)
 
 subsubsection "Post-fixed point computation"
+
+definition iter_widen :: "('a acom \<Rightarrow> 'a acom) \<Rightarrow> 'a acom \<Rightarrow> ('a::WN)acom option"
+where "iter_widen f = while_option (\<lambda>c. \<not> f c \<sqsubseteq> c) (\<lambda>c. c \<nabla>\<^sub>c f c)"
 
 definition
   prefp :: "(('a::preord) \<Rightarrow> 'a) \<Rightarrow> 'a \<Rightarrow> 'a option" where
 "prefp f = while_option (\<lambda>x. \<not> x \<sqsubseteq> f x) f"
 
+
 definition
   pfp_WN :: "(('a::WN)option acom \<Rightarrow> 'a option acom) \<Rightarrow> com \<Rightarrow> 'a option acom option"
-where "pfp_WN f c = (case lpfp\<^isub>c (\<lambda>c. c \<nabla>\<^sub>c f c) c of None \<Rightarrow> None
+where "pfp_WN f c = (case iter_widen f (\<bottom>\<^sub>c c) of None \<Rightarrow> None
                      | Some c' \<Rightarrow> prefp (\<lambda>c. c \<triangle>\<^sub>c f c) c')"
 
 lemma strip_map2_acom:
  "strip c1 = strip c2 \<Longrightarrow> strip(map2_acom f c1 c2) = strip c1"
 by(induct f c1 c2 rule: map2_acom.induct) simp_all
 
-lemma lpfp_step_up_pfp:
- "\<lbrakk> \<forall>c. strip(f c) = strip c;  lpfp\<^isub>c (\<lambda>c. c \<nabla>\<^sub>c f c) c = Some c' \<rbrakk> \<Longrightarrow> f c' \<sqsubseteq> c'"
-by (metis (no_types) assms lpfpc_pfp le_trans widen2_acom)
+lemma iter_widen_pfp: "iter_widen f c = Some c' \<Longrightarrow> f c' \<sqsubseteq> c'"
+by(auto simp add: iter_widen_def dest: while_option_stop)
+
+lemma strip_while: fixes f :: "'a acom \<Rightarrow> 'a acom"
+assumes "\<forall>c. strip (f c) = strip c" and "while_option P f c = Some c'"
+shows "strip c' = strip c"
+using while_option_rule[where P = "\<lambda>c'. strip c' = strip c", OF _ assms(2)]
+by (metis assms(1))
+
+lemma strip_iter_widen: fixes f :: "'a::WN acom \<Rightarrow> 'a acom"
+assumes "\<forall>c. strip (f c) = strip c" and "iter_widen f c = Some c'"
+shows "strip c' = strip c"
+proof-
+  have "\<forall>c. strip(c \<nabla>\<^sub>c f c) = strip c" by (metis assms(1) strip_map2_acom)
+  from strip_while[OF this] assms(2) show ?thesis by(simp add: iter_widen_def)
+qed
 
 lemma iter_down_pfp: assumes "mono f" and "f x0 \<sqsubseteq> x0" 
 and "prefp (\<lambda>c. c \<triangle>\<^sub>c f c) x0 = Some x"
@@ -163,22 +200,15 @@ proof-
   show ?thesis by blast
 qed
 
-
 lemma pfp_WN_pfp:
-  "\<lbrakk> \<forall>c. strip (f c) = strip c;  mono f;  pfp_WN f c = Some c' \<rbrakk> \<Longrightarrow> f c' \<sqsubseteq> c'"
+  "\<lbrakk> mono f;  pfp_WN f c = Some c' \<rbrakk> \<Longrightarrow> f c' \<sqsubseteq> c'"
 unfolding pfp_WN_def
-by (auto dest: iter_down_pfp lpfp_step_up_pfp split: option.splits)
-
-lemma strip_while: fixes f :: "'a acom \<Rightarrow> 'a acom"
-assumes "\<forall>c. strip (f c) = strip c" and "while_option P f c = Some c'"
-shows "strip c' = strip c"
-using while_option_rule[where P = "\<lambda>c'. strip c' = strip c", OF _ assms(2)]
-by (metis assms(1))
+by (auto dest: iter_down_pfp iter_widen_pfp split: option.splits)
 
 lemma strip_pfp_WN:
   "\<lbrakk> \<forall>c. strip(f c) = strip c; pfp_WN f c = Some c' \<rbrakk> \<Longrightarrow> strip c' = c"
 apply(auto simp add: pfp_WN_def prefp_def split: option.splits)
-by (metis (no_types) strip_lpfpc strip_map2_acom strip_while)
+by (metis (no_types) strip_map2_acom strip_while strip_bot_acom strip_iter_widen)
 
 locale Abs_Int2 = Abs_Int1_mono
 where \<gamma>=\<gamma> for \<gamma> :: "'av::{WN,L_top_bot} \<Rightarrow> val set"
@@ -190,7 +220,7 @@ definition AI_WN :: "com \<Rightarrow> 'av st option acom option" where
 lemma AI_WN_sound: "AI_WN c = Some c' \<Longrightarrow> CS c \<le> \<gamma>\<^isub>c c'"
 proof(simp add: CS_def AI_WN_def)
   assume 1: "pfp_WN (step' \<top>) c = Some c'"
-  from pfp_WN_pfp[OF allI[OF strip_step'] mono_step'2 1]
+  from pfp_WN_pfp[OF mono_step'2 1]
   have 2: "step' \<top> c' \<sqsubseteq> c'" .
   have 3: "strip (\<gamma>\<^isub>c (step' \<top> c')) = c" by(simp add: strip_pfp_WN[OF _ 1])
   have "lfp (step UNIV) c \<le> \<gamma>\<^isub>c (step' \<top> c')"
@@ -237,5 +267,244 @@ text{* Now all the analyses terminate: *}
 value [code] "show_acom_opt (AI_ivl' test4_ivl)"
 value [code] "show_acom_opt (AI_ivl' test5_ivl)"
 value [code] "show_acom_opt (AI_ivl' test6_ivl)"
+
+
+subsubsection "Termination: Intervals"
+
+(* interesting(?) relic
+lemma widen_assoc:
+  "~ (y::ivl) \<sqsubseteq> x \<Longrightarrow> ~ z \<sqsubseteq> x \<nabla> y \<Longrightarrow> ((x::ivl) \<nabla> y) \<nabla> z = x \<nabla> (y \<nabla> z)"
+apply(cases x)
+apply(cases y)
+apply(cases z)
+apply(rename_tac x1 x2 y1 y2 z1 z2)
+apply(simp add: le_ivl_def)
+apply(case_tac x1)
+apply(case_tac x2)
+apply(simp add:le_option_def widen_ivl_def split: if_splits option.splits)
+apply(simp add:le_option_def widen_ivl_def split: if_splits option.splits)
+apply(case_tac x2)
+apply(simp add:le_option_def widen_ivl_def split: if_splits option.splits)
+apply(case_tac y1)
+apply(case_tac y2)
+apply(simp add:le_option_def widen_ivl_def split: if_splits option.splits)
+apply(case_tac z1)
+apply(auto simp add:le_option_def widen_ivl_def split: if_splits option.splits ivl.splits)[1]
+apply(auto simp add:le_option_def widen_ivl_def split: if_splits option.splits ivl.splits)[1]
+apply(case_tac y2)
+apply(auto simp add:le_option_def widen_ivl_def split: if_splits option.splits ivl.splits)[1]
+apply(case_tac z1)
+apply(auto simp add:le_option_def widen_ivl_def split: if_splits ivl.splits option.splits)[1]
+apply(case_tac z2)
+apply(auto simp add:le_option_def widen_ivl_def split: if_splits option.splits)[1]
+apply(auto simp add:le_option_def widen_ivl_def split: if_splits option.splits)[1]
+done
+
+lemma widen_step_trans:
+  "~ (y::ivl) \<sqsubseteq> x \<Longrightarrow> ~ z \<sqsubseteq> x \<nabla> y \<Longrightarrow> EX u. (x \<nabla> y) \<nabla> z = x \<nabla> u \<and> ~ u \<sqsubseteq> x"
+by (metis widen_assoc preord_class.le_trans widen1)
+*)
+
+definition m_ivl :: "ivl \<Rightarrow> nat" where
+"m_ivl ivl = (case ivl of I l h \<Rightarrow>
+     (case l of None \<Rightarrow> 0 | Some _ \<Rightarrow> 1) + (case h of None \<Rightarrow> 0 | Some _ \<Rightarrow> 1))"
+
+lemma m_ivl_height: "m_ivl ivl \<le> 2"
+by(simp add: m_ivl_def split: ivl.split option.split)
+
+lemma m_ivl_anti_mono: "(y::ivl) \<sqsubseteq> x \<Longrightarrow> m_ivl x \<le> m_ivl y"
+by(auto simp: m_ivl_def le_option_def le_ivl_def
+        split: ivl.split option.split if_splits)
+
+lemma less_m_ivl_widen:
+  "~ y \<sqsubseteq> x \<Longrightarrow> m_ivl(x \<nabla> y) < m_ivl x"
+by(auto simp: m_ivl_def widen_ivl_def le_option_def le_ivl_def
+        split: ivl.splits option.splits if_splits)
+
+lemma Top_less_ivl: "\<top> \<sqsubseteq> x \<Longrightarrow> m_ivl x = 0"
+by(auto simp: m_ivl_def le_option_def le_ivl_def empty_def Top_ivl_def
+        split: ivl.split option.split if_splits)
+
+
+subsubsection "Termination: Abstract State"
+
+definition "m_st m st = (\<Sum>x\<in>set(dom st). m(fun st x))"
+
+lemma m_st_height: assumes "finite X" and "set (dom S) \<subseteq> X"
+shows "m_st m_ivl S \<le> 2 * card X"
+proof(auto simp: m_st_def)
+  have "(\<Sum>x\<in>set(dom S). m_ivl (fun S x)) \<le> (\<Sum>x\<in>set(dom S). 2)" (is "?L \<le> _")
+    by(rule setsum_mono)(simp add:m_ivl_height)
+  also have "\<dots> \<le> (\<Sum>x\<in>X. 2)"
+    by(rule setsum_mono3[OF assms]) simp
+  also have "\<dots> = 2 * card X" by(simp add: setsum_constant)
+  finally show "?L \<le> \<dots>" .
+qed
+
+lemma m_st_anti_mono:
+  "S1 \<sqsubseteq> S2 \<Longrightarrow> m_st m_ivl S2 \<le> m_st m_ivl S1"
+proof(auto simp: m_st_def le_st_def lookup_def split: if_splits)
+  let ?X = "set(dom S1)" let ?Y = "set(dom S2)"
+  let ?f = "fun S1" let ?g = "fun S2"
+  assume asm: "\<forall>x\<in>?Y. (x \<in> ?X \<longrightarrow> ?f x \<sqsubseteq> ?g x) \<and> (x \<in> ?X \<or> \<top> \<sqsubseteq> ?g x)"
+  hence 1: "\<forall>y\<in>?Y\<inter>?X. m_ivl(?g y) \<le> m_ivl(?f y)" by(simp add: m_ivl_anti_mono)
+  have 0: "\<forall>x\<in>?Y-?X. m_ivl(?g x) = 0" using asm by (auto simp: Top_less_ivl)
+  have "(\<Sum>y\<in>?Y. m_ivl(?g y)) = (\<Sum>y\<in>(?Y-?X) \<union> (?Y\<inter>?X). m_ivl(?g y))"
+    by (metis Un_Diff_Int)
+  also have "\<dots> = (\<Sum>y\<in>?Y-?X. m_ivl(?g y)) + (\<Sum>y\<in>?Y\<inter>?X. m_ivl(?g y))"
+    by(subst setsum_Un_disjoint) auto
+  also have "(\<Sum>y\<in>?Y-?X. m_ivl(?g y)) = 0" using 0 by simp
+  also have "0 + (\<Sum>y\<in>?Y\<inter>?X. m_ivl(?g y)) = (\<Sum>y\<in>?Y\<inter>?X. m_ivl(?g y))" by simp
+  also have "\<dots> \<le> (\<Sum>y\<in>?Y\<inter>?X. m_ivl(?f y))"
+    by(rule setsum_mono)(simp add: 1)
+  also have "\<dots> \<le> (\<Sum>y\<in>?X. m_ivl(?f y))"
+    by(simp add: setsum_mono3[of "?X" "?Y Int ?X", OF _ Int_lower2])
+  finally show "(\<Sum>y\<in>?Y. m_ivl(?g y)) \<le> (\<Sum>x\<in>?X. m_ivl(?f x))"
+    by (metis add_less_cancel_left)
+qed
+
+lemma less_m_st_widen:
+assumes "\<not> S2 \<sqsubseteq> S1" shows "m_st m_ivl (S1 \<nabla> S2) < m_st m_ivl S1"
+proof-
+  { let ?X = "set(dom S1)" let ?Y = "set(dom S2)"
+    let ?f = "fun S1" let ?g = "fun S2"
+    fix x assume "x \<in> ?X" "\<not> lookup S2 x \<sqsubseteq> ?f x"
+    have "(\<Sum>x\<in>?X\<inter>?Y. m_ivl(?f x \<nabla> ?g x)) < (\<Sum>x\<in>?X. m_ivl(?f x))" (is "?L < ?R")
+    proof cases
+      assume "x : ?Y"
+      have "?L < (\<Sum>x\<in>?X\<inter>?Y. m_ivl(?f x))"
+      proof(rule setsum_strict_mono1, simp)
+        show "\<forall>x\<in>?X\<inter>?Y. m_ivl(?f x \<nabla> ?g x) \<le> m_ivl (?f x)"
+          by (metis m_ivl_anti_mono widen1)
+      next
+        show "\<exists>x\<in>?X\<inter>?Y. m_ivl(?f x \<nabla> ?g x) < m_ivl(?f x)"
+          using `x:?X` `x:?Y` `\<not> lookup S2 x \<sqsubseteq> ?f x`
+          by (metis IntI less_m_ivl_widen lookup_def)
+      qed
+      also have "\<dots> \<le> ?R" by(simp add: setsum_mono3[OF _ Int_lower1])
+      finally show ?thesis .
+    next
+      assume "x ~: ?Y"
+      have "?L \<le> (\<Sum>x\<in>?X\<inter>?Y. m_ivl(?f x))"
+      proof(rule setsum_mono, simp)
+        fix x assume "x:?X \<and> x:?Y" show "m_ivl(?f x \<nabla> ?g x) \<le> m_ivl (?f x)"
+          by (metis m_ivl_anti_mono widen1)
+      qed
+      also have "\<dots> < m_ivl(?f x) + \<dots>"
+        using less_m_ivl_widen[OF `\<not> lookup S2 x \<sqsubseteq> ?f x`]
+        by (metis Nat.le_refl add_strict_increasing gr0I not_less0)
+      also have "\<dots> = (\<Sum>y\<in>insert x (?X\<inter>?Y). m_ivl(?f y))"
+        using `x ~: ?Y` by simp
+      also have "\<dots> \<le> (\<Sum>x\<in>?X. m_ivl(?f x))"
+        by(rule setsum_mono3)(insert `x:?X`, auto)
+      finally show ?thesis .
+    qed
+  } with assms show ?thesis
+    by(auto simp: le_st_def widen_st_def m_st_def Int_def)
+qed
+
+
+subsubsection "Termination: Option"
+
+definition "m_o m n opt = (case opt of None \<Rightarrow> n+1 | Some x \<Rightarrow> m x)"
+
+lemma m_o_anti_mono: "finite X \<Longrightarrow> domo S2 \<subseteq> X \<Longrightarrow> S1 \<sqsubseteq> S2 \<Longrightarrow>
+  m_o (m_st m_ivl) (2 * card X) S2 \<le> m_o (m_st m_ivl) (2 * card X) S1"
+apply(induction S1 S2 rule: le_option.induct)
+apply(auto simp: domo_def m_o_def m_st_anti_mono le_SucI m_st_height
+           split: option.splits)
+done
+
+lemma less_m_o_widen: "\<lbrakk> finite X; domo S2 \<subseteq> X; \<not> S2 \<sqsubseteq> S1 \<rbrakk> \<Longrightarrow>
+  m_o (m_st m_ivl) (2 * card X) (S1 \<nabla> S2) < m_o (m_st m_ivl) (2 * card X) S1"
+by(auto simp: m_o_def domo_def m_st_height less_Suc_eq_le less_m_st_widen
+        split: option.split)
+
+
+lemma domo_widen_subset: "domo (S1 \<nabla> S2) \<subseteq> domo S1 \<union> domo S2"
+apply(induction S1 S2 rule: widen_option.induct)
+apply (auto simp: domo_def widen_st_def)
+done
+
+subsubsection "Termination: Commands"
+
+lemma strip_widen_acom:
+  "strip c' = strip (c::'a::WN acom) \<Longrightarrow>  strip (c \<nabla>\<^sub>c c') = strip c"
+by(induction "widen::'a\<Rightarrow>'a\<Rightarrow>'a" c c' rule: map2_acom.induct) simp_all
+
+lemma annos_widen_acom[simp]: "strip c1 = strip (c2::'a::WN acom) \<Longrightarrow>
+  annos(c1 \<nabla>\<^sub>c c2) = map (%(x,y).x\<nabla>y) (zip (annos c1) (annos(c2::'a::WN acom)))"
+by(induction "widen::'a\<Rightarrow>'a\<Rightarrow>'a" c1 c2 rule: map2_acom.induct)
+  (simp_all add: size_annos_same2)
+
+lemma Com_widen_acom: "strip c2 = strip c1 \<Longrightarrow>
+  c1 : Com X \<Longrightarrow> c2 : Com X \<Longrightarrow> (c1 \<nabla>\<^sub>c c2) : Com X"
+apply(auto simp add: Com_def split: option.splits)
+apply(rename_tac S S' x)
+apply(erule in_set_zipE)
+apply(simp add: domo_def)
+apply (auto split: option.splits)
+apply(case_tac S)
+apply(case_tac S')
+apply simp
+apply fastforce
+apply(case_tac S')
+apply fastforce
+apply (fastforce simp: widen_st_def)
+done
+
+definition "m_c m c = (let as = annos c in \<Sum>i=0..<size as. m(as!i))"
+
+lemma measure_m_c: "finite X \<Longrightarrow> {(c, c \<nabla>\<^sub>c c') |c c'\<Colon>ivl st option acom.
+     strip c' = strip c \<and> c : Com X \<and> c' : Com X \<and> \<not> c' \<sqsubseteq> c}\<inverse>
+    \<subseteq> measure(m_c(m_o (m_st m_ivl) (2*card(X))))"
+apply(auto simp: m_c_def Let_def Com_def)
+apply(subgoal_tac "length(annos c') = length(annos c)")
+prefer 2 apply (simp add: size_annos_same2)
+apply (auto)
+apply(rule setsum_strict_mono1)
+apply simp
+apply (clarsimp)
+apply(erule m_o_anti_mono)
+apply(rule subset_trans[OF domo_widen_subset])
+apply fastsimp
+apply(rule widen1)
+apply(auto simp: le_iff_le_annos listrel_iff_nth)
+apply(rule_tac x=n in bexI)
+prefer 2 apply simp
+apply(erule less_m_o_widen)
+apply (simp)+
+done
+
+
+subsubsection "Termination: Post-Fixed Point Iterations"
+
+lemma iter_widen_termination:
+fixes c0 :: "'a::WN acom"
+assumes P_f: "\<And>c. P c \<Longrightarrow> P(f c)"
+assumes P_widen: "\<And>c c'. P c \<Longrightarrow> P c' \<Longrightarrow> P(c \<nabla>\<^sub>c c')"
+and "wf({(c::'a acom,c \<nabla>\<^sub>c c')|c c'. P c \<and> P c' \<and> ~ c' \<sqsubseteq> c}^-1)"
+and "P c0" and "c0 \<sqsubseteq> f c0" shows "EX c. iter_widen f c0 = Some c"
+proof(simp add: iter_widen_def, rule wf_while_option_Some[where P = "P"])
+  show "wf {(cc', c). (P c \<and> \<not> f c \<sqsubseteq> c) \<and> cc' = c \<nabla>\<^sub>c f c}"
+    apply(rule wf_subset[OF assms(3)]) by(blast intro: P_f)
+next
+  show "P c0" by(rule `P c0`)
+next
+  fix c assume "P c" thus "P (c \<nabla>\<^sub>c f c)" by(simp add: P_f P_widen)
+qed
+
+lemma
+  "EX c::ivl st option acom. iter_widen (step_ivl \<top>) (\<bottom>\<^sub>c c0) = Some c"
+apply(rule iter_widen_termination[where
+  P = "%c. strip c = c0 \<and> c : Com(vars c0)"])
+apply (simp_all add: strip_step' step'_Com Com_widen_acom strip_widen_acom bot_acom domo_Top)
+apply(rule wf_subset)
+apply(rule wf_measure)
+apply(rule subset_trans)
+prefer 2
+apply(rule measure_m_c[where X = "vars c0", OF finite_cvars])
+apply blast
+done
 
 end
